GMLInit/Meta/Basic.lean
@@ -37,26 +37,26 @@ macro "exfalso" : tactic => `(tactic| apply False.elim)
 
 macro "absurd " h:term : tactic => `(tactic| first | apply absurd _ $h | apply absurd $h)
 
-syntax "whnf" (&"lhs" <|> &"rhs")? (location)? : tactic
-macro_rules
-| `(tactic| whnf $[at $h:ident]?) =>
-  `(tactic| conv $[at $h]? => whnf)
-| `(tactic| whnf lhs $[at $h:ident]?) =>
-  `(tactic| conv $[at $h]? => {lhs; whnf})
-| `(tactic| whnf rhs $[at $h:ident]?) =>
-  `(tactic| conv $[at $h]? => {rhs; whnf})
+-- syntax "whnf" (&"lhs" <|> &"rhs")? (location)? : tactic
+-- macro_rules
+-- | `(tactic| whnf $[at $h:ident]?) =>
+--   `(tactic| conv $[at $h]? => whnf)
+-- | `(tactic| whnf lhs $[at $h:ident]?) =>
+--   `(tactic| conv $[at $h]? => {lhs; whnf})
+-- | `(tactic| whnf rhs $[at $h:ident]?) =>
+--   `(tactic| conv $[at $h]? => {rhs; whnf})
 
 def Tactic.constr (mvarId : MVarId) : MetaM (List MVarId) := do
-  withMVarContext mvarId do
-    checkNotAssigned mvarId `constr
-    let target ← getMVarType' mvarId
+  mvarId.withContext do
+    mvarId.checkNotAssigned `constr
+    let target ← mvarId.getType'
     matchConstStruct target.getAppFn
       (fun _ => throwTacticEx `constr mvarId "target is not an inductive datatype with one constructor")
       fun _ us cval => do
         let ctor := mkAppN (Lean.mkConst cval.name us) target.getAppArgs[:cval.numParams]
         let ctorType ← inferType ctor
         let (mvars, _, _) ← forallMetaTelescopeReducing ctorType (some cval.numFields)
-        apply mvarId <| mkAppN ctor mvars
+        mvarId.apply <| mkAppN ctor mvars
 
 elab "constr" : tactic => Tactic.withMainContext do
   let gs ← Tactic.constr (← Tactic.getMainGoal)
@@ -64,14 +64,14 @@ elab "constr" : tactic => Tactic.withMainContext do
   Tactic.replaceMainGoal gs
 
 def Tactic.left (mvarId : MVarId) : MetaM (List MVarId) := do
-  withMVarContext mvarId do
-    checkNotAssigned mvarId `left
-    let target ← getMVarType' mvarId
+  mvarId.withContext do
+    mvarId.checkNotAssigned `left
+    let target ← mvarId.getType'
     matchConstInduct target.getAppFn
       (fun _ => throwTacticEx `left mvarId "target is not an inductive datatype")
       fun ival us => do
         match ival.ctors with
-        | [ctor,_] => apply mvarId (mkConst ctor us)
+        | [ctor,_] => mvarId.apply (mkConst ctor us)
         | _ => throwTacticEx `left mvarId "target is not an inductive datatype with two constructors"
 
 elab "left" : tactic => Tactic.withMainContext do
@@ -80,14 +80,14 @@ elab "left" : tactic => Tactic.withMainContext do
   Tactic.replaceMainGoal gs
 
 def Tactic.right (mvarId : MVarId) : MetaM (List MVarId) := do
-  withMVarContext mvarId do
-    checkNotAssigned mvarId `right
-    let target ← getMVarType' mvarId
+  mvarId.withContext do
+    mvarId.checkNotAssigned `right
+    let target ← mvarId.getType'
     matchConstInduct target.getAppFn
       (fun _ => throwTacticEx `right mvarId "target is not an inductive datatype")
       fun ival us => do
         match ival.ctors with
-        | [_,ctor] => apply mvarId (mkConst ctor us)
+        | [_,ctor] => mvarId.apply (mkConst ctor us)
         | _ => throwTacticEx `right mvarId "target is not an inductive datatype with two constructors"
 
 elab "right" : tactic => Tactic.withMainContext do
