GMLInit/Data/List/LList.lean
@@ -5,11 +5,15 @@ import GMLInit.Data.Nat
 
 def LList (α) (n : Nat) := HList (List.replicate n α)
 
+@[matchPattern] protected def LList.nil {α} : LList α 0 := HList.nil
+
+@[matchPattern] protected def LList.cons {α n} (a : α) : LList α n → LList α (n+1) := HList.cons a
+
+def List.toLList {α} : (xs : List α) → LList α xs.length
+| [] => LList.nil
+| x::xs => LList.cons x (toLList xs)
+
 namespace LList
-
-@[matchPattern] protected def nil {α} : LList α 0 := HList.nil
-
-@[matchPattern] protected def cons {α n} (a : α) : LList α n → LList α (n+1) := HList.cons a
 
 scoped infixr:67 " :: " => LList.cons
 scoped syntax (name := llist) "[" term,* "]"  : term
