GMLInit/Data/Nat/Sub.lean
@@ -52,17 +52,20 @@ protected theorem add_sub_cancel_right (x y : Nat) : (x + y) - y = x := by
 protected theorem add_sub_comm (x y : Nat) : x + (y - x) = y + (x - y) := by
   induction x, y with
   | left x => 
-    calc
+    calc 
+    _ = x + (0 - x) := rfl
     _ = x + 0 := by rw [Nat.zero_sub]
     _ = 0 + x := by rw [Nat.add_comm]
     _ = 0 + (x - 0) := by rw [Nat.sub_zero]
   | right y => 
     calc
+    _ = 0 + (y - 0) := rfl
     _ = 0 + y := by rw [Nat.sub_zero]
     _ = y + 0 := by rw [Nat.add_comm]
     _ = y + (0 - y) := by rw [Nat.zero_sub]
   | diag x y H =>
     calc
+    _ = (x + 1) + ((y + 1) - (x + 1)) := rfl
     _ = (x + 1) + (y - x) := by rw [Nat.succ_sub_succ']
     _ = (x + (y - x)) + 1 := by rw [Nat.succ_add']
     _ = (y + (x - y)) + 1 := by rw [H]
