GMLInit/Prelude.lean
@@ -1,5 +1,8 @@
 import Lean
 
+instance (α) [Subsingleton α] : DecidableEq α 
+| _, _ => isTrue (Subsingleton.allEq _ _)
+
 infix:50 " ≅ " => HEq
 
 class Inv (α : Type _) where
